qed commit_staged!

proof/ktcore_proof/agree.v
@@ -17,25 +17,26 @@ Collection W := sem.
 
 Definition kt_ptsto γ ep uid opt_pk : iProp Σ :=
   ∃ dig,
-  "#Hlook_dig" ∷ mono_list_idx_own γ.(cfg.digs)
+  "#Hidx_dig" ∷ mono_list_idx_own γ.(cfg.digs)
     (ep - γ.(cfg.info).(digs_info.start_ep)) dig ∗
   "%Heq_pk" ∷ ⌜last $ ktcore.to_pks γ.(cfg.vrf_pk) uid dig = opt_pk⌝.
 
-Definition is_staged γcli uid keys_start_ep keys : iProp Σ :=
+(* [start_ep] of [keys]. *)
+Definition is_staged_keys γcli uid start_ep keys : iProp Σ :=
   ∃ digs next_ver,
-  let n_drop := (keys_start_ep - γcli.(cfg.info).(digs_info.start_ep))%nat in
+  let n_drop := (start_ep - γcli.(cfg.info).(digs_info.start_ep))%nat in
   "#Hlb_digs" ∷ mono_list_lb_own γcli.(cfg.digs) digs ∗
-  "%Hstaged" ∷ ⌜is_staged_keys γcli.(cfg.vrf_pk) (drop n_drop digs)
+  "%Hstaged" ∷ ⌜staged_keys γcli.(cfg.vrf_pk) (drop n_drop digs)
     uid keys next_ver⌝ ∗
 
-  "%Hlt_start" ∷ ⌜γcli.(cfg.info).(digs_info.start_ep) ≤ keys_start_ep⌝.
+  "%Hlt_start" ∷ ⌜γcli.(cfg.info).(digs_info.start_ep) ≤ start_ep⌝.
 
-Definition is_audit γcli γadtr end_ep : iProp Σ :=
+Definition is_audit γcli γadtr ep : iProp Σ :=
   ∃ (digs : list $ list w8),
   "#Hcli_digs" ∷ mono_list_lb_own γcli.(cfg.digs) digs ∗
   "#Hadtr_digs" ∷ mono_list_lb_own γadtr.(cfg.digs) digs ∗
   "%Hlen_digs" ∷ ⌜Z.of_nat $ length digs =
-    S end_ep - γcli.(cfg.info).(digs_info.start_ep)⌝ ∗
+    S ep - γcli.(cfg.info).(digs_info.start_ep)⌝ ∗
   "%Hmono_plain" ∷ ⌜mono_plain γadtr.(cfg.vrf_pk)
     (drop γadtr.(cfg.info).(digs_info.audit_offset) digs)⌝ ∗
 
@@ -62,26 +63,73 @@ Lemma kt_ptsto_agree γ ep uid opt_pk0 opt_pk1 :
   ⌜opt_pk0 = opt_pk1⌝.
 Proof.
   iNamedSuffix 1 "0". iNamedSuffix 1 "1".
-  iDestruct (mono_list_idx_agree with "Hlook_dig0 Hlook_dig1") as %->.
+  iDestruct (mono_list_idx_agree with "Hidx_dig0 Hidx_dig1") as %->.
   by subst.
 Qed.
 
-Lemma kt_ptsto_txfer γcli γadtr ep uid opt_pk end_ep :
+Lemma kt_ptsto_txfer γcli γadtr ep uid opt_pk audit_ep :
   γcli ↪KT[ep, uid] opt_pk -∗
-  is_audit γcli γadtr end_ep -∗
-  ⌜(γadtr.(cfg.info).(digs_info.start_ep) +
-    γadtr.(cfg.info).(digs_info.audit_offset) ≤ ep ≤ end_ep)%nat⌝ -∗
+  is_audit γcli γadtr audit_ep -∗
+  ⌜γadtr.(cfg.info).(digs_info.start_ep) +
+    γadtr.(cfg.info).(digs_info.audit_offset) ≤ ep ≤ audit_ep⌝ -∗
   γadtr ↪KT[ep, uid] opt_pk.
 Proof.
   iIntros "@@%". rewrite /kt_ptsto.
   eremember (ep - _)%nat as ep_t.
   list_elem digs ep_t as dig'. subst.
   iDestruct (mono_list_idx_own_get with "Hcli_digs") as "Hlook"; [done|].
-  iDestruct (mono_list_idx_agree with "Hlook_dig Hlook") as %<-.
+  iDestruct (mono_list_idx_agree with "Hidx_dig Hlook") as %<-.
   iClear "Hlook".
   iDestruct (mono_list_idx_own_get with "Hadtr_digs") as "Hlook"; [done|].
   rewrite Heq_vrf Heq_start.
   by iFrame "#".
+Qed.
+
+Lemma commit_staged γcli uid keys_start_ep keys γadtr audit_ep :
+  is_staged_keys γcli uid keys_start_ep keys -∗
+  is_audit γcli γadtr audit_ep -∗
+  ⌜γadtr.(cfg.info).(digs_info.start_ep) +
+    γadtr.(cfg.info).(digs_info.audit_offset) ≤ keys_start_ep⌝ -∗
+  ⌜keys_start_ep + length keys ≤ S audit_ep⌝ -∗
+  (∀ i opt_pk,
+    let ep := (keys_start_ep + i)%nat in
+    ⌜keys !! i = Some opt_pk⌝ -∗
+    γadtr ↪KT[ep, uid] opt_pk).
+Proof.
+  iIntros "@ #Haudit %% * %Hlook_keys".
+  apply lookup_lt_Some in Hlook_keys as ?.
+  iApply kt_ptsto_txfer; [|done|word].
+  iNamed "Haudit". rewrite /kt_ptsto.
+  destruct Hstaged as (?&Hlast_digs&_&?&Hstaged).
+  rewrite last_lookup in Hlast_digs.
+  apply lookup_lt_Some in Hlast_digs.
+  autorewrite with len in *.
+  iAssert (⌜digs `prefix_of` digs0⌝)%I as %(adtr_digs&->).
+  { iDestruct (mono_list_lb_valid with "Hlb_digs Hcli_digs")
+      as %[?|Hpref]; [done|].
+    by apply prefix_length_eq in Hpref as ->; [|lia]. }
+  iClear "Hcli_digs Hadtr_digs".
+  autorewrite with len in *.
+
+  odestruct (Hstaged _) as (_&->).
+  { rewrite drop_app_le in Hmono_plain; [|word].
+    eremember (keys_start_ep - _)%nat as n_drop.
+    rewrite -(take_drop
+      (n_drop - γadtr.(cfg.info).(digs_info.audit_offset))
+      (drop _ _)) drop_drop in Hmono_plain.
+    replace (_ + _)%nat with n_drop in Hmono_plain; [|lia].
+    list_simplifier.
+    rewrite /mono_plain !fmap_app in Hmono_plain |-*.
+    apply list_reln_app in Hmono_plain as [_ Hmono].
+    apply list_reln_app in Hmono as [Hmono _].
+    by rewrite Heq_vrf. }
+  clear Hstaged.
+
+  apply list_lookup_fmap_Some in Hlook_keys as (dig&->&Hlook_digs).
+  iExists _. iSplit; [|done].
+  iApply mono_list_idx_own_get; [|done].
+  rewrite lookup_drop in Hlook_digs.
+  exact_eq Hlook_digs. f_equal. lia.
 Qed.
 
 End proof.
